generic/Zeta.GenericVerifier.fst
@@ -50,3 +50,25 @@ let update_record_set_valid
                      gk = AppK ak /\
                      gv = AppV (S.index ws i))))
   = admit()
+
+let runapp_doesnot_change_nonref_slots
+  (#vspec: verifier_spec)
+  (e: verifier_log_entry vspec {is_appfn e})
+  (vs: vspec.vtls_t)
+  (s: vspec.slot_t)
+  : Lemma (requires (let RunApp _ _ ss = e in
+                     vspec.valid (verify_step e vs) /\ not (S.mem s ss)))
+          (ensures (let vs' = verify_step e vs in
+                    vspec.get s vs == vspec.get s vs'))
+  = admit()
+
+let runapp_doesnot_change_slot_emptiness
+  (#vspec: verifier_spec)
+  (e: verifier_log_entry vspec {is_appfn e})
+  (vs: vspec.vtls_t)
+  (s: vspec.slot_t)
+  : Lemma (requires (let RunApp _ _ ss = e in
+                     vspec.valid (verify_step e vs)))
+          (ensures (let vs' = verify_step e vs in
+                    (None = vspec.get s vs) <==> (None = vspec.get s vs')))
+  = admit()
