generic/Zeta.Generic.Interleave.fsti
@@ -97,6 +97,13 @@ val lemma_non_cur_thread_state_extend (#vspec: verifier_spec) (#n:_) (tid: nat{t
                     let st_post = thread_state_post tid il i in
                     st_pre == st_post))
 
+val lemma_thread_state_prefix (#vspec: verifier_spec) (#n:_)
+  (il: verifiable_log vspec n) (i:seq_index il)
+  : Lemma (ensures (let t,j = i2s_map il i in
+                    let tl = G.index (to_glog il) t in
+                    cur_thread_state_pre il i == T.state_pre tl j))
+          [SMTPat (cur_thread_state_pre il i)]
+
 let is_blum_add (#vspec #n:_) (il: verifiable_log vspec n) (i: seq_index il)
   : bool
   = let ti = i2s_map il i in
